theories/fundamental.v
@@ -9,11 +9,6 @@ Section fundamental.
   Implicit Types w : (leibnizC Word).
   Implicit Types interp : D.
 
-(* "Hmtr" : [∗ map] r0↦w ∈ <[PC:=inr (RX, g, b, e, a)]> r, r0 ↦ᵣ w
-  "Hmta" : [∗ map] a0↦w ∈ m, a0 ↦ₐ w *)
-
-  (* Lemma extract_a m (a : Addr) : *)
-  (*   [∗ map] a0↦w ∈ m, a0 ↦ₐ w -∗  *)
 
   Lemma extract_r_ex reg (r : RegName) :
     (∃ w, reg !! r = Some w) →
@@ -36,7 +31,154 @@ Section fundamental.
     iSpecialize ("Hmap" with "[Hw]"); eauto. 
     iSpecialize ("Hupdate" with "[Hmap]"); eauto.
   Qed.
-    
+
+  Lemma key_non_dupl γ : ∀ q, own γ 1%Qp ∗ own γ q%Qp -∗ False.
+  Proof.
+    iIntros (q) "[H1 Hq]".
+    iDestruct (own_valid_2 γ with "[H1] [Hq]") as "%"; iFrame.
+    iPureIntro. rewrite frac.frac_op' in H2.
+    assert (((1 + q)%Qp ≤ 1%Qp)%Qc).
+      by apply frac.frac_valid'.
+    by apply (Qp_not_plus_q_ge_1 q). 
+  Qed.
+
+
+  Lemma fundamental_RX_global b e γ (a : Addr) :
+    (read_cond b e Global γ interp -∗
+    ⟦ inr ((RX,Global),b,e,a) ⟧ₑ )%I. 
+  Proof.
+    iIntros "#Hinv".
+    iIntros (r m) "Hreg".
+    iExists _,_,_,_,_; iSplit; eauto; simpl.
+    iIntros "Hmreg /=".
+    iLöb as "IH". 
+    iApply (wp_bind (fill [SeqCtx])).
+    destruct (decide (isCorrectPC (inr ((RX,Global),b,e,a)))). 
+    - (* Correct PC *)
+      iInv (logN.@(b, e)) as (ws) "HregionHvalid" "Hcls".
+      iDestruct (extract_from_region _ _ a with "HregionHvalid")
+        as (w) "(Hregionl & Hvalidl & >Ha & Hva & Hregionh & Hvalidh)".
+      { admit. }
+      { admit. }
+      { admit. } (* a + -1 and a + 1 are some addresses *)
+      iDestruct (extract_r (<[PC:=inr (RX, Global, b, e, a)]> r) PC
+                           (inr (RX, Global, b, e, a))
+                   with "[Hmreg]") as "[HPC HPCmap]";
+        first by apply (lookup_insert r PC). iFrame.
+      destruct (cap_lang.decode w) eqn:Hi. (* proof by cases on each instruction *)
+      + admit. (* Jmp *)
+      + admit. (* Jnz *)
+      + admit. (* Mov *)
+      + (* Load *)
+        (* these come from the reg interp relation *)
+        iAssert (∃ w, dst ↦ᵣ w)%I as (wdst) "Hdst"; [admit|].
+        iAssert (∃ w, src ↦ᵣ w)%I as (wsrc) "Hsrc"; [admit|].
+        destruct wsrc eqn:Hsrc; [admit|].
+        destruct c. do 3 destruct p.
+        iAssert (∃ w, a0 ↦ₐ w)%I as (wa0) "Ha0"; [admit|].
+        
+        iApply (wp_load_success with "[HPC Hdst Hsrc Ha Ha0]"); eauto.
+        * admit.
+        * admit.
+        * admit.
+        * iFrame.
+        * iNext. iIntros "(HPC & Hdst & Ha) /=".
+          iApply (wp_wand with "[HPC Hreg HPCmap]").
+          { iApply wp_pure_step_later; eauto. iNext.
+            iApply ("IH" with "Hreg").
+            iSpecialize ("HPCmap" with "HPC"). rewrite insert_insert. iFrame. 
+          } iAssert (∀ v : val cap_lang,
+                        (λ _ : valC cap_lang, ∃ r0 : Reg, registers_mapsto r0) v
+                                -∗ ∃ r0 : Reg, registers_mapsto r0)%I as "Htrivial".
+          { iIntros (_) "Hreg". iFrame. } iFrame. 
+          iApply "Hcls". iNext. admit. 
+      + admit. (* Store *)
+      + admit. (* Lt *)
+      + admit. (* Add *)
+      + admit. (* Sub *)
+      + admit. (* Lea *)
+      + admit. (* Restrict *)
+      + admit. (* Subseg *)
+      + admit. (* IsPtr *)
+      + admit. (* GetL *)
+      + admit. (* GetP *)
+      + admit. (* GetB *)
+      + admit. (* GetE *)
+      + admit. (* GetA *)
+      + admit. (* Fail *)
+      + admit. (* Halt *)   
+    - (* Incorrect PC *) admit.
+  Admitted. 
+
+  Lemma fundamental_RX_local b e γ (a : Addr) :
+    (read_cond b e Local γ interp -∗
+    ⟦ inr ((RX,Local),b,e,a) ⟧ₑ )%I. 
+  Proof.
+    iIntros "#Hinv".
+    iIntros (r m) "Hreg".
+    iExists _,_,_,_,_; iSplit; eauto; simpl.
+    iExists γ. iIntros "Hkey Hmreg /=".
+    iLöb as "IH". 
+    iApply (wp_bind (fill [SeqCtx])).
+    destruct (decide (isCorrectPC (inr ((RX,Local),b,e,a)))). 
+    - (* Correct PC *)
+      iInv (logN.@(b, e)) as "[HregionHvalid | >Hkey']" "Hcls";
+        last by iDestruct (key_non_dupl γ with "[Hkey Hkey']") as "Hf"; iFrame.
+      iDestruct "HregionHvalid" as (ws) "HregionHvalid". 
+      iDestruct (extract_from_region _ _ a with "HregionHvalid")
+        as (w) "(Hregionl & Hvalidl & >Ha & Hva & Hregionh & Hvalidh)".
+      { admit. }
+      { admit. }
+      { admit. } (* a + -1 and a + 1 are some addresses *)
+      iDestruct (extract_r (<[PC:=inr (RX, Local, b, e, a)]> r) PC
+                           (inr (RX, Local, b, e, a))
+                   with "[Hmreg]") as "[HPC HPCmap]";
+        first by apply (lookup_insert r PC). iFrame.
+      destruct (cap_lang.decode w) eqn:Hi. (* proof by cases on each instruction *)
+      + admit. (* Jmp *)
+      + admit. (* Jnz *)
+      + admit. (* Mov *)
+      + (* Load *)
+        (* these come from the reg interp relation *)
+        iAssert (∃ w, dst ↦ᵣ w)%I as (wdst) "Hdst"; [admit|].
+        iAssert (∃ w, src ↦ᵣ w)%I as (wsrc) "Hsrc"; [admit|].
+        destruct wsrc eqn:Hsrc; [admit|].
+        destruct c. do 3 destruct p.
+        iAssert (∃ w, a0 ↦ₐ w)%I as (wa0) "Ha0"; [admit|].
+        
+        iApply (wp_load_success with "[HPC Hdst Hsrc Ha Ha0]"); eauto.
+        * admit.
+        * admit.
+        * admit.
+        * iFrame.
+        * iNext. iIntros "(HPC & Hdst & Ha) /=".
+          iApply (wp_wand with "[HPC Hreg HPCmap Hkey]").
+          { iApply wp_pure_step_later; eauto. iNext.
+            iApply ("IH" with "Hreg Hkey").
+            iSpecialize ("HPCmap" with "HPC"). rewrite insert_insert. iFrame. 
+          } iAssert (∀ v : val cap_lang,
+                        (λ _ : valC cap_lang, ∃ r0 : Reg, registers_mapsto r0) v
+                         -∗ ∃ r0 : Reg, registers_mapsto r0)%I as "Htrivial".
+          { iIntros (_) "Hreg". iFrame. } iFrame. 
+          iApply "Hcls". iNext. iLeft. admit. 
+      + admit. (* Store *)
+      + admit. (* Lt *)
+      + admit. (* Add *)
+      + admit. (* Sub *)
+      + admit. (* Lea *)
+      + admit. (* Restrict *)
+      + admit. (* Subseg *)
+      + admit. (* IsPtr *)
+      + admit. (* GetL *)
+      + admit. (* GetP *)
+      + admit. (* GetB *)
+      + admit. (* GetE *)
+      + admit. (* GetA *)
+      + admit. (* Fail *)
+      + admit. (* Halt *)   
+    - (* Incorrect PC *) admit.
+  Admitted. 
+  
   Theorem fundamental (perm : Perm) b e g γ (a : Addr) :
     (⌜perm = RX⌝ ∧ read_cond b e g γ interp)%I ∨
     (⌜perm = RWX⌝ ∧ read_cond b e g γ interp ∧
@@ -45,74 +187,12 @@ Section fundamental.
      write_cond b e g γ interp (λne w, True%I))%I -∗
     ⟦ inr ((perm,g),b,e,a) ⟧ₑ.
   Proof. 
-    iIntros "[#[-> Hrc] | [#(Hrwx & Hrc & Hwc) | #(Hwlx & Hrc & Hwc)]]".
+    iIntros "[#[-> Hinv] | [#(Hrwx & Hrc & Hwc) | #(Hwlx & Hrc & Hwc)]]".
     - destruct g.
       + (* Global *)
-        iIntros (r m) "Hreg". iIntros "Hmreg /=".
-        iLöb as "IH". 
-        iApply (wp_bind (fill [SeqCtx])).
-        destruct (decide (isCorrectPC (inr ((RX,Global),b,e,a)))). 
-        { (* Correct PC *)
-          (* iDestruct (extract_r (<[PC:=inr (RX, Global, b, e, a)]> r) PC *)
-          (*                      (inr (RX, Global, b, e, a)) *)
-          (*              with "[Hmreg]") as "[HPC HPCmap]"; *)
-          (*   first by apply (lookup_insert r PC). iFrame. *)
-          iDestruct "Hrc" as (b' e') "#[[% %] Hinv]".
-          iInv (logN.@(b', e')) as (ws) "HregionHvalid" "Hcls".
-          iDestruct (extract_from_region _ _ a with "HregionHvalid")
-            as (w) "(Hregionl & Hvalidl & >Ha & Hva & Hregionh & Hvalidh)".
-          { apply (in_range_is_correctPC RX Global b e); auto. }
-          { admit. } { admit. } (* a + -1 and a + 1 are some addresses *)
-          iDestruct (extract_r (<[PC:=inr (RX, Global, b, e, a)]> r) PC
-                               (inr (RX, Global, b, e, a))
-                       with "[Hmreg]") as "[HPC HPCmap]";
-            first by apply (lookup_insert r PC). iFrame.
-          destruct (cap_lang.decode w) eqn:Hi. (* proof by cases on each instruction *)
-          - admit. (* Jmp *)
-          - admit. (* Jnz *)
-          - admit. (* Mov *)
-          - (* Load *)
-            (* these come from the reg interp relation *)
-            iAssert (∃ w, dst ↦ᵣ w)%I as (wdst) "Hdst"; [admit|].
-            iAssert (∃ w, src ↦ᵣ w)%I as (wsrc) "Hsrc"; [admit|].
-            destruct wsrc eqn:Hsrc; [admit|].
-            destruct c. do 3 destruct p.
-            iAssert (∃ w, a0 ↦ₐ w)%I as (wa0) "Ha0"; [admit|].
-            
-            iApply (wp_load_success with "[HPC Hdst Hsrc Ha Ha0]"); eauto.
-            + admit.
-            + admit.
-            + admit.
-            + iFrame.
-            + iNext. iIntros "(HPC & Hdst & Ha) /=".
-              iApply (wp_wand with "[HPC Hreg HPCmap]").
-              { iApply wp_pure_step_later; eauto. iNext.
-                iApply ("IH" with "Hreg").
-                iSpecialize ("HPCmap" with "HPC"). rewrite insert_insert. iFrame. 
-              } iAssert (∀ v : val cap_lang,
-                                (λ _ : valC cap_lang, ∃ r0 : Reg, registers_mapsto r0) v
-                                -∗ ∃ r0 : Reg, registers_mapsto r0)%I as "Htrivial".
-              { iIntros (_) "Hreg". iFrame. } iFrame. 
-              iApply "Hcls". iNext. admit. 
-           - admit. (* Store *)
-          - admit. (* Lt *)
-          - admit. (* Add *)
-          - admit. (* Sub *)
-          - admit. (* Lea *)
-          - admit. (* Restrict *)
-          - admit. (* Subseg *)
-          - admit. (* IsPtr *)
-          - admit. (* GetL *)
-          - admit. (* GetP *)
-          - admit. (* GetB *)
-          - admit. (* GetE *)
-          - admit. (* GetA *)
-          - admit. (* Fail *)
-          - admit. (* Halt *)
-        } 
-        { (* Incorrect PC *) admit. }
+          by iApply fundamental_RX_global. 
       + (* Local *)
-        admit.
+          by iApply fundamental_RX_local. 
     - (* read and write condition, non local *) admit. 
     - (* read and write condition, permit local *) admit. 
 Admitted. 
